examples/t2/Clang.v
@@ -1,0 +1,83 @@
+From ExtLib Require
+  Structures.Maps.
+From ExtLib Require Import Data.String.
+
+From Coq Require Import
+  ZArith.ZArith
+  Strings.String.
+
+From CTree Require Import
+  CTree.Core
+  CTree.Interp.State
+  CTree.Events.State
+  CTree.Events.Writer.
+
+Generalizable All Variables.
+
+Import Ctree CTreeNotations.
+Local Open Scope ctl_scope.
+Local Open Scope ctree_scope.
+Local Open Scope Z_scope.
+
+Generalizable All Variables.
+
+Module Clang.
+  Module M := Maps.
+  Context `{MM: @M.Map string Z Ctx}.
+  Definition Mem := stateE Ctx.
+
+  Definition assert(k: string)(p: Z -> Prop)(m: Ctx): Prop :=
+    match M.lookup k m with
+    | Some v => p v
+    | None => False
+    end.
+  
+  Definition load(k: string): ctree Mem Z :=
+    m <- get ;;
+    match M.lookup k m with
+    | Some v => Ret v
+    | None => Ret 0%Z
+    end.
+
+  Definition store(k: string) (v: Z): ctree Mem unit :=
+    m <- get ;;    
+    put (M.add k v m).
+
+  (* a := f b *)
+  Definition update(a: string) (b: string) (f: Z -> Z): ctree Mem unit :=
+    m <- get ;;
+    match M.lookup b m with
+    | Some v => put (M.add a (f v) m)
+    | None => put (M.add a (f 0%Z) m)
+    end.
+  
+  Declare Scope clang_scope.
+  Local Open Scope clang_scope.
+  Declare Custom Entry clang.
+  
+  Notation "[[ e ]]" := e (at level 0, e custom clang at level 95) : clang_scope.
+  Notation "( x )" := x (in custom clang, x at level 99) : clang_scope.
+  Notation "{ x }" := x (in custom clang at level 0, x constr): clang_scope.
+  Notation "x" := x (in custom clang at level 0, x constr at level 0) : clang_scope.
+
+  Notation "x := c" := (store x c)
+                         (in custom clang at level 60, right associativity) : clang_scope.
+  
+  Notation "x ::= y '+' c" := (update x y (fun z => z + c))
+                                (in custom clang at level 60, right associativity) : clang_scope.
+  
+  Notation "x ::= y '-' c" := (update x y (fun z => z - c))
+                                (in custom clang at level 60, right associativity) : clang_scope.
+  
+  Notation "'while' c '?>' z 'do' b 'done'" :=
+    (@Ctree.iter _ _ unit unit
+       (fun 'tt =>
+          x <- load c;;
+          if x >? z then
+            b ;; continue
+          else
+            break
+       ) tt) (in custom clang at level 63): ctree_scope.
+
+  Notation "t1 ;;; t2" := (Ctree.bind t1 (fun _ => t2)) (in custom clang at level 62, right associativity): clang_scope.
+End Clang.
